Split Steel.Memory into further little modules

pulse/ulib/experimental/Steel.Memory.fsti
@@ -37,59 +37,7 @@ val upd_joined_heap: (m:mem) -> (h:heap{m_disjoint m h}) -> mem
 
 let hmem (fp:hprop) = m:mem{interp (fp `star` locks_invariant m) (heap_of_mem m)}
 
-////////////////////////////////////////////////////////////////////////////////
-// Actions:
-// sel, split, update
-////////////////////////////////////////////////////////////////////////////////
-let pre_action (fp:hprop) (a:Type) (fp':a -> hprop) =
-  hheap fp -> (x:a & hheap (fp' x))
 
-let is_frame_preserving #a #fp #fp' (f:pre_action fp a fp') =
-  forall frame h0.
-    interp (fp `star` frame) h0 ==>
-    (let (| x, h1 |) = f h0 in
-     interp (fp' x `star` frame) h1)
-
-let action_depends_only_on_fp (#pre:_) (#a:_) (#post:_) (f:pre_action pre a post)
-  = forall (h0:hheap pre)
-      (h1:heap {disjoint h0 h1})
-      (post: (x:a -> fp_prop (post x))).
-      (interp pre (join h0 h1) /\ (
-       let (| x0, h |) = f h0 in
-       let (| x1, h' |) = f (join h0 h1) in
-       x0 == x1 /\
-       (post x0 h <==> post x1 h')))
-
-let action (fp:hprop) (a:Type) (fp':a -> hprop) =
-  f:pre_action fp a fp'{ is_frame_preserving f /\
-                         action_depends_only_on_fp f }
-
-
-let pre_m_action (fp:hprop) (a:Type) (fp':a -> hprop) =
-  hmem fp -> (x:a & hmem (fp' x))
-
-val m_action_depends_only_on (#pre:hprop) (#a:Type) (#post:a -> hprop) (f:pre_m_action pre a post) : prop
-
-val is_m_frame_preserving (#a:Type) (#fp:hprop) (#fp':a -> hprop) (f:pre_m_action fp a fp') : prop
-
-let m_action (fp:hprop) (a:Type) (fp':a -> hprop) =
-  f:pre_m_action fp a fp'{ is_m_frame_preserving f /\ m_action_depends_only_on f }
-
-val frame_fp_prop (#fp:_) (#a:Type) (#fp':_) (act:action fp a fp')
-                  (#frame:hprop) (q:fp_prop frame)
-   : Lemma (forall (h0:hheap (fp `star` frame)).
-              (affine_star fp frame h0;
-               q h0 ==>
-               (let (| x, h1 |) = act h0 in
-                q h1)))
-
-val sel (#a:_) (r:ref a) (m:hheap (ptr r))
-  : a
-
-/// sel respect pts_to
-val sel_lemma (#a:_) (r:ref a) (p:permission) (m:hheap (ptr_perm r p))
-  : Lemma (interp (ptr r) m /\
-           interp (pts_to r p (sel r m)) m)
 
 /// memories satisfying [p1 `star` p2] can be split
 /// into disjoint fragments satisfying each of them
@@ -98,29 +46,3 @@ val split_mem (p1 p2:hprop) (m:hheap (p1 `star` p2))
             let m1, m2 = ms in
             disjoint m1 m2 /\
             m == join m1 m2})
-
-/// upd requires a full permission
-val upd (#a:_) (r:ref a) (v:a)
-  : m_action (ptr_perm r full_permission) unit (fun _ -> pts_to r full_permission v)
-
-
-val upd_array
-  (#t:_)
-  (a:array_ref t)
-  (iseq: Seq.lseq t (U32.v (length a)))
-  (i:U32.t{U32.v i < U32.v (length a)})
-  (v: t)
-  : m_action
-    (pts_to_array a full_permission iseq)
-    unit
-    (fun _ -> pts_to_array a full_permission (Seq.upd iseq (U32.v i) v))
-
-
-
-val alloc (#a:_) (v:a)
-  : m_action emp (ref a) (fun x -> pts_to x full_permission v)
-
-val lock (p:hprop) : Type0
-
-val new_lock (p:hprop)
-  : m_action p (lock p) (fun _ -> emp)
