pulse/ulib/experimental/Steel.Actions.Array.fsti
@@ -1,0 +1,36 @@
+(*
+   Copyright 2019 Microsoft Research
+
+   Licensed under the Apache License, Version 2.0 (the "License");
+   you may not use this file except in compliance with the License.
+   You may obtain a copy of the License at
+
+       http://www.apache.org/licenses/LICENSE-2.0
+
+   Unless required by applicable law or agreed to in writing, software
+   distributed under the License is distributed on an "AS IS" BASIS,
+   WITHOUT WARRANTIES OR CONDITIONS OF ANY KIND, either express or implied.
+   See the License for the specific language governing permissions and
+   limitations under the License.
+*)
+module Steel.Actions.Array
+open Steel.Heap
+open Steel.HProp
+open Steel.Memory
+open FStar.Real
+open Steel.Permissions
+open Steel.Actions
+module U32 = FStar.UInt32
+
+
+
+val upd_array
+  (#t:_)
+  (a:array_ref t)
+  (iseq: Seq.lseq t (U32.v (length a)))
+  (i:U32.t{U32.v i < U32.v (length a)})
+  (v: t)
+  : m_action
+    (pts_to_array a full_permission iseq)
+    unit
+    (fun _ -> pts_to_array a full_permission (Seq.upd iseq (U32.v i) v))
