pulse/ulib/experimental/Steel.Actions.Locks.fst
@@ -1,0 +1,262 @@
+(*
+   Copyright 2019 Microsoft Research
+
+   Licensed under the Apache License, Version 2.0 (the "License");
+   you may not use this file except in compliance with the License.
+   You may obtain a copy of the License at
+
+       http://www.apache.org/licenses/LICENSE-2.0
+
+   Unless required by applicable law or agreed to in writing, software
+   distributed under the License is distributed on an "AS IS" BASIS,
+   WITHOUT WARRANTIES OR CONDITIONS OF ANY KIND, either express or implied.
+   See the License for the specific language governing permissions and
+   limitations under the License.
+*)
+module Steel.Actions.Locks
+open Steel.Heap
+open Steel.HProp
+open FStar.Real
+open Steel.Permissions
+module U32 = FStar.UInt32
+open Steel.Actions
+open FStar.FunctionalExtensionality
+
+friend Steel.Heap
+friend Steel.HProp
+friend Steel.Memory
+friend Steel.Actions
+#set-options "--initial_fuel 1 --max_fuel 1 --initial_ifuel 0 --max_ifuel 0"
+
+
+let lock (p:hprop) = nat
+
+module L = FStar.List.Tot
+
+let new_lock_pre_m_action (p:hprop)
+  : pre_m_action p (lock p) (fun _ -> emp)
+  = fun m ->
+     let l = Available p in
+     let locks' = l :: m.locks in
+     assert (interp (lock_store_invariant locks') (heap_of_mem m));
+     let mem :mem = { m with locks = locks' } in
+     assert (locks_invariant mem == p `star` locks_invariant m);
+     assert (interp (locks_invariant mem) (heap_of_mem mem));
+     emp_unit (locks_invariant mem);
+     star_commutative emp (locks_invariant mem);
+     assert (interp (emp `star` locks_invariant mem) (heap_of_mem mem));
+     let lock_id = List.Tot.length locks' - 1 in
+     (| lock_id, mem |)
+
+let emp_unit_left (p:hprop)
+  : Lemma
+    ((emp `star` p) `equiv` p)
+  = emp_unit p;
+    star_commutative emp p
+
+let equiv_star_left (p q r:hprop)
+  : Lemma
+    (requires q `equiv` r)
+    (ensures (p `star` q) `equiv` (p `star` r))
+  = ()
+
+#push-options "--warn_error -271 --max_fuel 2 --initial_fuel 2"
+let new_lock_is_frame_preserving (p:hprop)
+  : Lemma (is_m_frame_preserving (new_lock_pre_m_action p))
+  = let aux (frame:hprop) (m:hmem (p `star` frame))
+      : Lemma
+          (ensures (
+            let (| x, m1 |) = new_lock_pre_m_action p m in
+            interp (emp `star` frame `star` locks_invariant m1) (heap_of_mem m1)))
+          [SMTPat ()]
+      = let (| x, m1 |) = new_lock_pre_m_action p m in
+        assert (m1.locks == Available p :: m.locks);
+        assert (locks_invariant m1 == (p `star` locks_invariant m));
+        assert (interp ((p `star` frame) `star` locks_invariant m) (heap_of_mem m));
+        star_associative p frame (locks_invariant m);
+        assert (interp (p `star` (frame `star` locks_invariant m)) (heap_of_mem m));
+        star_commutative frame (locks_invariant m);
+        equiv_star_left p (frame `star` locks_invariant m) (locks_invariant m `star` frame);
+        assert (interp (p `star` (locks_invariant m `star` frame)) (heap_of_mem m));
+        star_associative p (locks_invariant m) frame;
+        assert (interp ((p `star` locks_invariant m) `star` frame) (heap_of_mem m));
+        assert (interp ((locks_invariant m1) `star` frame) (heap_of_mem m));
+        assert (heap_of_mem m == heap_of_mem m1);
+        star_commutative (locks_invariant m1) frame;
+        assert (interp (frame `star` (locks_invariant m1)) (heap_of_mem m1));
+        emp_unit_left (frame `star` (locks_invariant m1));
+        assert (interp (emp `star` (frame `star` (locks_invariant m1))) (heap_of_mem m1));
+        star_associative emp frame (locks_invariant m1)
+    in
+    ()
+#pop-options
+
+let new_lock (p:hprop)
+  : m_action p (lock p) (fun _ -> emp)
+  = new_lock_is_frame_preserving p;
+    new_lock_pre_m_action p
+
+////////////////////////////////////////////////////////////////////////////////
+assume
+val get_lock (l:lock_store) (i:nat{i < L.length l})
+  : (prefix : lock_store &
+     li : lock_state &
+     suffix : lock_store {
+       l == L.(prefix @ (li::suffix)) /\
+       L.length (li::suffix) == i + 1
+     })
+
+let lock_i (l:lock_store) (i:nat{i < L.length l}) : lock_state =
+  let (| _, li, _ |) = get_lock l i in
+  li
+
+assume
+val lock_store_invariant_append (l1 l2:lock_store)
+  : Lemma (lock_store_invariant (l1 @ l2) `equiv`
+           (lock_store_invariant l1 `star` lock_store_invariant l2))
+
+let hprop_of_lock_state (l:lock_state) : hprop =
+  match l with
+  | Available p -> p
+  | Locked p -> p
+
+let lock_ok (#p:hprop) (l:lock p) (m:mem) =
+  l < L.length m.locks /\
+  hprop_of_lock_state (lock_i m.locks l) == p
+
+let lock_store_evolves : Preorder.preorder lock_store =
+  fun (l1 l2 : lock_store) ->
+    L.length l2 >= L.length l1 /\
+    (forall (i:nat{i < L.length l1}).
+       hprop_of_lock_state (lock_i l1 i) ==
+       hprop_of_lock_state (lock_i l2 i))
+
+let mem_evolves : Preorder.preorder mem =
+  fun m0 m1 -> lock_store_evolves m0.locks m1.locks
+
+let lock_ok_stable (#p:_) (l:lock p) (m0 m1:mem)
+  : Lemma (lock_ok l m0 /\
+           m0 `mem_evolves` m1 ==>
+           lock_ok l m1)
+  = ()
+
+let pure (p:prop) : hprop = refine emp (fun _ -> p)
+
+#push-options "--max_fuel 2 --initial_fuel 2 --max_ifuel 1 --initial_ifuel 1"
+let intro_pure (p:prop) (q:hprop) (h:hheap q { p })
+  : hheap (pure p `star` q)
+  = emp_unit q;
+    star_commutative q emp;
+    h
+#pop-options
+
+#push-options "--max_fuel 2 --initial_fuel 2 --max_ifuel 1 --initial_ifuel 1"
+let intro_hmem_or (p:prop) (q:hprop) (h:hmem q)
+  : hmem (h_or (pure p) q)
+  = h
+#pop-options
+
+let middle_to_head (p q r:hprop) (h:hheap (p `star` (q `star` r)))
+  : hheap (q `star` (p `star` r))
+  = star_associative p q r;
+    star_commutative p q;
+    star_associative q p r;
+    h
+
+#push-options "--max_fuel 2 --initial_fuel 2 --max_ifuel 1 --initial_ifuel 1"
+let maybe_acquire #p (l:lock p) (m:mem { lock_ok l m } )
+  : (b:bool &
+     m:hmem (h_or (pure (b == false)) p))
+  = let (| prefix, li, suffix |) = get_lock m.locks l in
+    match li with
+    | Available _ ->
+      let h = heap_of_mem m in
+      assert (interp (lock_store_invariant m.locks) h);
+      lock_store_invariant_append prefix (li::suffix);
+      assert (lock_store_invariant m.locks `equiv`
+             (lock_store_invariant prefix `star`
+                      (p `star` lock_store_invariant suffix)));
+      assert (interp (lock_store_invariant prefix `star`
+                       (p `star` lock_store_invariant suffix)) h);
+      let h = middle_to_head (lock_store_invariant prefix) p (lock_store_invariant suffix) h in
+      assert (interp (p `star`
+                        (lock_store_invariant prefix `star`
+                         lock_store_invariant suffix)) h);
+      let new_lock_store = prefix @ (Locked p :: suffix) in
+      lock_store_invariant_append prefix (Locked p :: suffix);
+      assert (lock_store_invariant new_lock_store `equiv`
+              (lock_store_invariant prefix `star`
+                         lock_store_invariant suffix));
+      equiv_star_left p (lock_store_invariant new_lock_store)
+                        (lock_store_invariant prefix `star`
+                          lock_store_invariant suffix);
+      assert (interp (p `star` lock_store_invariant new_lock_store) h);
+      let h : hheap (p `star` lock_store_invariant new_lock_store) = h in
+      assert (heap_of_mem m == h);
+      star_commutative p (lock_store_invariant new_lock_store);
+      affine_star (lock_store_invariant new_lock_store) p h;
+      assert (interp (lock_store_invariant new_lock_store) h);
+      let mem : hmem p = { m with locks = new_lock_store } in
+      let b = true in
+      let mem : hmem (h_or (pure (b==false)) p) = intro_hmem_or (b == false) p mem in
+      (| b, mem |)
+
+    | Locked _ ->
+      let b = false in
+      assert (interp (pure (b == false)) (heap_of_mem m));
+      let h : hheap (locks_invariant m) = heap_of_mem m in
+      let h : hheap (pure (b==false) `star` locks_invariant m) =
+        intro_pure (b==false) (locks_invariant m) h in
+      intro_or_l (pure (b==false) `star` locks_invariant m)
+                 (p `star` locks_invariant m)
+                 h;
+      or_star (pure (b==false)) p (locks_invariant m) h;
+      assert (interp (h_or (pure (b==false)) p `star` locks_invariant m) h);
+      (| false, m |)
+#pop-options
+
+#push-options "--max_fuel 2 --initial_fuel 2 --max_ifuel 1 --initial_ifuel 1"
+let hmem_emp (p:hprop) (m:hmem p) : hmem emp = m
+#pop-options
+
+#push-options "--max_fuel 2 --initial_fuel 2 --max_ifuel 1 --initial_ifuel 1 --z3rlimit 20"
+let release #p (l:lock p) (m:hmem p { lock_ok l m } )
+  : (b:bool &
+     hmem emp)
+  = let (| prefix, li, suffix |) = get_lock m.locks l in
+    let h = heap_of_mem m in
+    lock_store_invariant_append prefix (li::suffix);
+    assert (interp (p `star`
+                     (lock_store_invariant prefix `star`
+                       (lock_store_invariant (li::suffix)))) h);
+    match li with
+    | Available _ ->
+      (* this case is odd, but not inadmissible.
+         We're releasing a lock that was not previously acquired.
+         We could either fail, or just silently proceed.
+         I choose to at least signal this case in the result
+         so that we can decide to fail if we like, at a higher layer.
+
+         Another cleaner way to handle this would be to insist
+         that lockable resources are non-duplicable ...
+         in which case this would be unreachable, since we have `p star p` *)
+      (| false, hmem_emp p m |)
+
+    | Locked _ ->
+      assert (interp (p `star`
+                        (lock_store_invariant prefix `star`
+                          (lock_store_invariant suffix))) h);
+      let h = middle_to_head p (lock_store_invariant prefix) (lock_store_invariant suffix) h in
+      assert (interp (lock_store_invariant prefix `star`
+                        (p `star`
+                          (lock_store_invariant suffix))) h);
+      let new_lock_store = prefix @ (Available p :: suffix) in
+      lock_store_invariant_append prefix (Available p :: suffix);
+      assert (lock_store_invariant new_lock_store `equiv`
+                (lock_store_invariant prefix `star`
+                 (p `star` lock_store_invariant (suffix))));
+      assert (interp (lock_store_invariant new_lock_store) h);
+      emp_unit_left (lock_store_invariant new_lock_store);
+      let mem : hmem emp = { m with locks = new_lock_store } in
+      (| true, mem |)
+#pop-options
