pulse/ulib/experimental/Steel.Actions.Pointer.fst
@@ -1,0 +1,381 @@
+(*
+   Copyright 2019 Microsoft Research
+
+   Licensed under the Apache License, Version 2.0 (the "License");
+   you may not use this file except in compliance with the License.
+   You may obtain a copy of the License at
+
+       http://www.apache.org/licenses/LICENSE-2.0
+
+   Unless required by applicable law or agreed to in writing, software
+   distributed under the License is distributed on an "AS IS" BASIS,
+   WITHOUT WARRANTIES OR CONDITIONS OF ANY KIND, either express or implied.
+   See the License for the specific language governing permissions and
+   limitations under the License.
+*)
+module Steel.Actions.Pointer
+open Steel.Heap
+open Steel.HProp
+open FStar.Real
+open Steel.Permissions
+module U32 = FStar.UInt32
+open Steel.Actions
+open FStar.FunctionalExtensionality
+
+friend Steel.Heap
+friend Steel.HProp
+friend Steel.Memory
+friend Steel.Actions
+
+#set-options "--initial_fuel 1 --max_fuel 1 --initial_ifuel 0 --max_ifuel 0"
+
+
+////////////////////////////////////////////////////////////////////////////////
+// sel
+////////////////////////////////////////////////////////////////////////////////
+#push-options "--max_fuel 3"
+let sel #a (r:ref a) (m:hheap (ptr r))
+  : a
+  = let Ref _ _ v = select_addr m r in
+    v
+#pop-options
+
+#push-options "--max_fuel 2"
+let sel_lemma #a (r:ref a) (p:permission) (m:hheap (ptr_perm r p))
+  = ()
+#pop-options
+
+
+let upd_heap #a (r:ref a) (v:a)
+  : pre_action (ptr_perm r full_permission) unit (fun _ -> pts_to r full_permission v)
+  = fun h -> (| (), update_addr h r (Ref a full_permission v) |)
+
+#push-options "--initial_fuel 2 --max_fuel 2 --initial_ifuel 1 --max_ifuel 1 --z3rlimit 10"
+let upd_lemma' (#a:_) (r:ref a) (v:a) (h:heap) (frame:hprop)
+  : Lemma
+    (requires
+      interp (ptr_perm r full_permission `star` frame) h)
+    (ensures (
+      let (| x, h1 |) = upd_heap r v h in
+      interp (pts_to r full_permission v `star` frame) h1))
+  = let aux (h0 h1:heap)
+     : Lemma
+       (requires
+         disjoint h0 h1 /\
+         h == join h0 h1 /\
+         interp (ptr_perm r full_permission) h0 /\
+         interp frame h1)
+       (ensures (
+         let (| _, h' |) = upd_heap r v h in
+         let h0' = update_addr h0 r (Ref a full_permission v) in
+         disjoint h0' h1 /\
+         interp (pts_to r full_permission v) h0' /\
+         interp frame h1 /\
+         h' == join h0' h1))
+       [SMTPat (disjoint h0 h1)]
+     = let (| _, h'|) = upd_heap r v h in
+       let h0' = update_addr h0 r (Ref a full_permission v) in
+       assume (disjoint h0' h1);  //AR: 12/11: TODO
+       mem_equiv_eq h' (join h0' h1)
+   in
+   ()
+#pop-options
+
+
+#push-options "--warn_error -271"
+let upd'_is_frame_preserving (#a:_) (r:ref a) (v:a)
+  : Lemma (is_frame_preserving (upd_heap r v))
+  = let aux (#a:_) (r:ref a) (v:a) (h:heap) (frame:hprop)
+      : Lemma
+        (requires
+          interp (ptr_perm r full_permission `star` frame) h)
+        (ensures (
+          let (| _, h1 |) = (upd_heap r v h) in
+          interp (pts_to r full_permission v `star` frame) h1))
+        [SMTPat ()]
+      = upd_lemma' r v h frame
+   in
+   ()
+#pop-options
+
+#push-options "--initial_fuel 2 --max_fuel 2 --initial_ifuel 1 --max_ifuel 1"
+let upd'_preserves_join #a (r:ref a) (v:a)
+                       (h0:hheap (ptr_perm r full_permission))
+                       (h1:heap {disjoint h0 h1})
+  : Lemma
+     (let (| x0, h |) = upd_heap r v h0 in
+      let (| x1, h' |) = upd_heap r v (join h0 h1) in
+      x0 == x1 /\
+      disjoint h h1 /\
+      h' == join h h1)
+  = let (| x0, h |) = upd_heap r v h0 in
+    let (| x1, h' |) = upd_heap r v (join h0 h1) in
+    assert (h == update_addr h0 r (Ref a full_permission v));
+    assert (h' == update_addr (join h0 h1) r (Ref a full_permission v));
+    assert (disjoint h h1);
+    assert (h' `mem_equiv` join h h1)
+#pop-options
+
+#push-options "--warn_error -271"
+let upd'_depends_only_on_fp #a (r:ref a) (v:a)
+  : Lemma (action_depends_only_on_fp (upd_heap r v))
+  =
+    let pre = ptr_perm r full_permission in
+    let post = pts_to r full_permission v in
+    let aux (h0:hheap pre)
+            (h1:heap {disjoint h0 h1})
+            (q:fp_prop post)
+    : Lemma
+      (let (| x0, h |) = upd_heap r v h0 in
+        let (| x1, h' |) = upd_heap r v (join h0 h1) in
+        x0 == x1 /\
+        (q h <==> q h'))
+      [SMTPat ()]
+    = let (| x0, h |) = upd_heap r v h0 in
+      let (| x1, h' |) = upd_heap r v (join h0 h1) in
+      assert (x0 == x1);
+      upd'_preserves_join r v h0 h1;
+      assert (h' == join h h1)
+    in
+    ()
+#pop-options
+
+#push-options "--z3rlimit 50 --max_fuel 2 --initial_fuel 2"
+let upd' #a (r:ref a) (v:a)
+  : pre_m_action (ptr_perm r full_permission) unit (fun _ -> pts_to r full_permission v)
+  = fun m ->
+      upd'_is_frame_preserving r v;
+      let (| _, h' |) = upd_heap r v m.heap in
+      let m':mem = {m with heap = h'} in
+      (| (), m' |)
+#pop-options
+
+#push-options "--warn_error -271 --initial_fuel 2 --max_fuel 2"
+let upd_is_frame_preserving (#a:_) (r:ref a) (v:a)
+  : Lemma (is_m_frame_preserving (upd' r v))
+  =
+  let aux (#a:_) (r:ref a) (v:a) (frame:hprop) (m:hmem (ptr_perm r full_permission `star` frame))
+      : Lemma
+        (ensures (
+          let (| _, m1 |) = upd' r v m in
+          interp (pts_to r full_permission v `star` frame `star` locks_invariant m1) m1.heap))
+        [SMTPat ()]
+      = star_associative (ptr_perm r full_permission) frame (locks_invariant m);
+        star_associative (pts_to r full_permission v) frame (locks_invariant m);
+        upd_lemma' r v m.heap (frame `star` locks_invariant m)
+   in
+   ()
+#pop-options
+
+#push-options "--warn_error -271"
+let upd_depends_only_on_fp (#a:_) (r:ref a) (v:a)
+  : Lemma (m_action_depends_only_on (upd' r v))
+  =
+    let pre = ptr_perm r full_permission in
+    let post = pts_to r full_permission v in
+    let aux (m0:hmem pre)
+            (h1:heap {m_disjoint m0 h1})
+            (q:fp_prop post)
+    : Lemma
+      (let (| x0, m |) = upd' r v m0 in
+       let (| x1, m' |) = upd' r v (upd_joined_heap m0 h1) in
+        x0 == x1 /\
+        (q (heap_of_mem m) <==> q (heap_of_mem m')))
+      [SMTPat ()]
+    = let (| x0, m |) = upd' r v m0 in
+      let (| x1, m' |) = upd' r v (upd_joined_heap m0 h1) in
+      upd'_preserves_join r v m0.heap h1;
+      assert (m'.heap == join m.heap h1)
+    in
+    ()
+#pop-options
+
+let upd #a (r:ref a) (v:a)
+  : m_action (ptr_perm r full_permission) unit (fun _ -> pts_to r full_permission v)
+  = upd_is_frame_preserving r v;
+    upd_depends_only_on_fp r v;
+    upd' r v
+
+val alloc' (#a:_) (v:a) (frame:hprop) (tmem:mem{interp frame (heap_of_mem tmem)})
+  : (x:ref a &
+     tmem:mem { interp (pts_to x full_permission v `star` frame) (heap_of_mem tmem)} )
+
+
+#push-options "--max_fuel 2 --initial_fuel 2 --initial_ifuel 1 --max_ifuel 1"
+let alloc' #a v frame m
+  = let x : ref a = m.ctr in
+    let cell = Ref a full_permission v in
+    let mem : heap = on _ (fun i -> if i = x then Some cell else None) in
+    assert (disjoint mem m.heap);
+    assert (mem `contains_addr` x);
+    assert (select_addr mem x == cell);
+    let mem' = join mem m.heap in
+    intro_pts_to x full_permission v mem;
+    assert (interp (pts_to x full_permission v) mem);
+    assert (interp frame m.heap);
+    intro_star (pts_to x full_permission v) frame mem m.heap;
+    assert (interp (pts_to x full_permission v `star` frame) mem');
+    let t = {
+      ctr = x + 1;
+      heap = mem';
+      locks = m.locks;
+      properties = ();
+    } in
+    (| x, t |)
+#pop-options
+
+let singleton_heap #a (x:ref a) (c:cell) : heap =
+    on _ (fun i -> if i = x then Some c else None)
+
+let singleton_pts_to #a (x:ref a) (c:cell{Ref? c})
+  : Lemma (requires (Ref?.a c == a))
+          (ensures (interp (pts_to x (Ref?.perm c) (Ref?.v c)) (singleton_heap x c)))
+  = ()
+
+#push-options "--max_fuel 2 --initial_fuel 2 --max_ifuel 1 --initial_ifuel 1 --z3rlimit 50"
+let alloc_pre_m_action (#a:_) (v:a)
+  : pre_m_action emp (ref a) (fun x -> pts_to x full_permission v)
+  = fun m ->
+    let x : ref a = m.ctr in
+    let cell = Ref a full_permission v in
+    let mem : heap = singleton_heap x cell in
+    assert (disjoint mem m.heap);
+    assert (mem `contains_addr` x);
+    assert (select_addr mem x == cell);
+    let mem' = join mem m.heap in
+    intro_pts_to x full_permission v mem;
+    assert (interp (pts_to x full_permission v) mem);
+    let frame = (lock_store_invariant m.locks) in
+    assert (interp frame m.heap);
+    intro_star (pts_to x full_permission v) frame mem m.heap;
+    assert (interp (pts_to x full_permission v `star` frame) mem');
+    let t = {
+      ctr = x + 1;
+      heap = mem';
+      locks = m.locks;
+      properties = ();
+    } in
+    (| x, t |)
+#pop-options
+
+#push-options "--z3rlimit 70 --max_fuel 2 --initial_fuel 2 --initial_ifuel 1 --max_ifuel 1"
+let alloc_is_frame_preserving' (#a:_) (v:a) (m:mem) (frame:hprop)
+  : Lemma
+    (requires
+      interp (frame `star` locks_invariant m) (heap_of_mem m))
+    (ensures (
+      let (| x, m1 |) = alloc_pre_m_action v m in
+      interp (pts_to x full_permission v `star` frame `star` locks_invariant m1) (heap_of_mem m1)))
+  = let (| x, m1 |) = alloc_pre_m_action v m in
+    assert (x == m.ctr);
+    assert (m1.ctr = m.ctr + 1);
+    assert (m1.locks == m.locks);
+    let h = heap_of_mem m in
+    let h1 = heap_of_mem m1 in
+    let cell = (Ref a full_permission v) in
+    assert (h1 == join (singleton_heap x cell) h);
+    intro_pts_to x full_permission v (singleton_heap x cell);
+    singleton_pts_to x cell;
+    assert (interp (pts_to x full_permission v) (singleton_heap x cell));
+    assert (interp (frame `star` locks_invariant m) h);
+    intro_star (pts_to x full_permission v) (frame `star` locks_invariant m) (singleton_heap x cell) h;
+    assert (interp (pts_to x full_permission v `star` (frame `star` locks_invariant m)) h1);
+    star_associative (pts_to x full_permission v) frame (locks_invariant m);
+    assert (interp (pts_to x full_permission v `star` frame `star` locks_invariant m) h1)
+#pop-options
+
+#push-options "--z3rlimit 150 --warn_error -271 --initial_fuel 2 --max_fuel 2"
+let alloc_is_frame_preserving (#a:_) (v:a)
+  : Lemma (is_m_frame_preserving (alloc_pre_m_action v))
+  = let aux (frame:hprop) (m:hmem (emp `star` frame))
+      : Lemma
+          (ensures (
+            let (| x, m1 |) = alloc_pre_m_action v m in
+            interp (pts_to x full_permission v `star` frame `star` locks_invariant m1) (heap_of_mem m1)))
+          [SMTPat ()]
+      = alloc_is_frame_preserving' v m frame
+    in
+    ()
+#pop-options
+
+#push-options "--z3rlimit 10 --max_fuel 2 --initial_fuel 2 --initial_ifuel 1 --max_ifuel 1"
+let alloc_preserves_disjoint (#a:_) (v:a) (m0:hmem emp) (h1:heap {m_disjoint m0 h1})
+  : Lemma (let (| x0, m |) = alloc_pre_m_action v m0 in
+           disjoint (heap_of_mem m) h1)
+  = let (| x0, m |) = alloc_pre_m_action v m0 in
+    let h0 = heap_of_mem m0 in
+    let h' = heap_of_mem m in
+    let aux (ad:addr) : Lemma (disjoint_addr h' h1 ad)
+      = if ad >= m0.ctr then ()
+        else begin
+          let h_alloc = singleton_heap #a m0.ctr (Ref a full_permission v) in
+          assert (h' == join h_alloc h0);
+          assert (h_alloc ad == None);
+         assert (h0 ad == h' ad);
+         assert (disjoint_addr h0 h1 ad)
+        end
+    in Classical.forall_intro aux
+#pop-options
+
+#push-options "--z3rlimit 30 --max_fuel 2 --initial_fuel 2 --max_ifuel 1 --initial_ifuel 1"
+let alloc_preserves_join (#a:_) (v:a) (m0:hmem emp) (h1:heap {m_disjoint m0 h1})
+  : Lemma (
+      let h0 = heap_of_mem m0 in
+      let h = join h0 h1 in
+      let m1:mem = { m0 with heap = h } in
+      let (| x0, m |) = (alloc_pre_m_action v) m0 in
+      let (| x1, m' |) = (alloc_pre_m_action v) m1 in
+      heap_of_mem m' == join (heap_of_mem m) h1)
+   = let h0 = heap_of_mem m0 in
+     let h = join h0 h1 in
+     let m1:mem = { m0 with heap = h } in
+     let (| x0, m |) = (alloc_pre_m_action v) m0 in
+     let (| x1, m' |) = (alloc_pre_m_action v) m1 in
+     let h_alloc = singleton_heap #a m0.ctr (Ref a full_permission v) in
+     // let hm = heap_of_mem m in
+     // let hm' = heap_of_mem m' in
+     // assert (hm == join h_alloc h0);
+     // assert (hm' == join h_alloc h);
+     // assert (hm' == join h_alloc (join h0 h1));
+     join_associative' h_alloc h0 h1
+#pop-options
+
+#push-options "--z3rlimit 10 --warn_error -271"
+let alloc_depends_only_on (#a:_) (v:a)
+  : Lemma (m_action_depends_only_on (alloc_pre_m_action v))
+  = let aux
+        (m0:hmem emp)
+        (h1:heap { m_disjoint m0 h1 })
+        (post:(x:ref a -> fp_prop (pts_to x full_permission v)))
+      : Lemma
+          (ensures (
+            let h0 = heap_of_mem m0 in
+            let h = join h0 h1 in
+            let m1 = { m0 with heap = h } in
+            let (| x0, m |) = (alloc_pre_m_action v) m0 in
+            let (| x1, m' |) = (alloc_pre_m_action v) m1 in
+            x0 == x1 /\
+            (post x0 (heap_of_mem m) <==> post x1 (heap_of_mem m'))))
+          [SMTPat ()]
+      =
+        let h0 = heap_of_mem m0 in
+        let h = join h0 h1 in
+        let m1 = { m0 with heap = h } in
+        let (| x0, m |) = (alloc_pre_m_action v) m0 in
+        let (| x1, m' |) = (alloc_pre_m_action v) m1 in
+        assert (x0 == x1);
+        alloc_preserves_disjoint v m0 h1;
+//        assert (disjoint (heap_of_mem m) h1);
+        affine_star (pts_to x0 full_permission v) (locks_invariant m) (heap_of_mem m);
+        alloc_preserves_join v m0 h1
+//        assert (interp (pts_to x0 full_permission v) (heap_of_mem m));
+//        assert (heap_of_mem m' == join (heap_of_mem m) h1)
+    in
+    ()
+#pop-options
+
+let alloc (#a:_) (v:a)
+  : m_action emp (ref a) (fun x -> pts_to x full_permission v)
+  = alloc_is_frame_preserving v;
+    alloc_depends_only_on v;
+    alloc_pre_m_action v
