pulse/ulib/experimental/Steel.Actions.Pointer.fsti
@@ -1,0 +1,41 @@
+(*
+   Copyright 2019 Microsoft Research
+
+   Licensed under the Apache License, Version 2.0 (the "License");
+   you may not use this file except in compliance with the License.
+   You may obtain a copy of the License at
+
+       http://www.apache.org/licenses/LICENSE-2.0
+
+   Unless required by applicable law or agreed to in writing, software
+   distributed under the License is distributed on an "AS IS" BASIS,
+   WITHOUT WARRANTIES OR CONDITIONS OF ANY KIND, either express or implied.
+   See the License for the specific language governing permissions and
+   limitations under the License.
+*)
+module Steel.Actions.Pointer
+open Steel.Heap
+open Steel.HProp
+open Steel.Memory
+open FStar.Real
+open Steel.Permissions
+open Steel.Actions
+module U32 = FStar.UInt32
+
+
+val sel (#a:_) (r:ref a) (m:hheap (ptr r))
+  : a
+
+/// sel respect pts_to
+val sel_lemma (#a:_) (r:ref a) (p:permission) (m:hheap (ptr_perm r p))
+  : Lemma (interp (ptr r) m /\
+           interp (pts_to r p (sel r m)) m)
+
+
+/// upd requires a full permission
+val upd (#a:_) (r:ref a) (v:a)
+  : m_action (ptr_perm r full_permission) unit (fun _ -> pts_to r full_permission v)
+
+
+val alloc (#a:_) (v:a)
+  : m_action emp (ref a) (fun x -> pts_to x full_permission v)
