pulse/ulib/experimental/Steel.Actions.fst
@@ -1,0 +1,76 @@
+(*
+   Copyright 2019 Microsoft Research
+
+   Licensed under the Apache License, Version 2.0 (the "License");
+   you may not use this file except in compliance with the License.
+   You may obtain a copy of the License at
+
+       http://www.apache.org/licenses/LICENSE-2.0
+
+   Unless required by applicable law or agreed to in writing, software
+   distributed under the License is distributed on an "AS IS" BASIS,
+   WITHOUT WARRANTIES OR CONDITIONS OF ANY KIND, either express or implied.
+   See the License for the specific language governing permissions and
+   limitations under the License.
+*)
+module Steel.Actions
+open Steel.Heap
+open Steel.HProp
+open FStar.Real
+open Steel.Permissions
+open Steel.Memory
+module U32 = FStar.UInt32
+open FStar.FunctionalExtensionality
+
+friend Steel.Memory
+
+#set-options "--initial_fuel 1 --max_fuel 1 --initial_ifuel 0 --max_ifuel 0"
+
+let m_action_depends_only_on #pre #a #post (f:pre_m_action pre a post)
+  = forall (m0:hmem pre)
+      (h1:heap {m_disjoint m0 h1})
+      (post: (x:a -> fp_prop (post x))).
+      (let m1 = upd_joined_heap m0 h1 in
+       let (| x0, m |) = f m0 in
+       let (| x1, m' |) = f m1 in
+       x0 == x1 /\
+       (post x0 (heap_of_mem m) <==> post x1 (heap_of_mem m')))
+
+#push-options "--initial_fuel 2 --max_fuel 2"
+let is_m_frame_preserving #a #fp #fp' (f:pre_m_action fp a fp') =
+  forall frame (m0:hmem (fp `star` frame)).
+    (affine_star fp frame (heap_of_mem m0);
+     let (| x, m1 |) = f m0 in
+     interp (fp' x `star` frame `star` locks_invariant m1) (heap_of_mem m1))
+#pop-options
+
+#push-options "--max_fuel 2 --initial_fuel 2 --z3rlimit 10"
+let frame_fp_prop' #fp #a #fp' frame
+                   (q:fp_prop frame)
+                   (act:action fp a fp')
+                   (h0:hheap (fp `star` frame))
+   : Lemma (requires q h0)
+           (ensures (
+             let (| x, h1 |) = act h0 in
+             q h1))
+   = assert (interp (Refine (fp `star` frame) q) h0);
+     assert (interp (fp `star` (Refine frame q)) h0);
+     let (| x, h1 |) = act h0 in
+     assert (interp (fp' x `star` (Refine frame q)) h1);
+     refine_star_r (fp' x) frame q;
+     assert (interp (Refine (fp' x `star` frame) q) h1);
+     assert (q h1)
+#pop-options
+
+let frame_fp_prop #fp #a #fp' (act:action fp a fp')
+                  (#frame:hprop) (q:fp_prop frame)
+   = let aux (h0:hheap (fp `star` frame))
+       : Lemma
+         (requires q h0)
+         (ensures
+           (let (|x, h1|) = act h0 in
+            q h1))
+         [SMTPat (act h0)]
+       = frame_fp_prop' frame q act h0
+     in
+     ()
