pulse/ulib/experimental/Steel.Actions.fsti
@@ -1,0 +1,68 @@
+(*
+   Copyright 2019 Microsoft Research
+
+   Licensed under the Apache License, Version 2.0 (the "License");
+   you may not use this file except in compliance with the License.
+   You may obtain a copy of the License at
+
+       http://www.apache.org/licenses/LICENSE-2.0
+
+   Unless required by applicable law or agreed to in writing, software
+   distributed under the License is distributed on an "AS IS" BASIS,
+   WITHOUT WARRANTIES OR CONDITIONS OF ANY KIND, either express or implied.
+   See the License for the specific language governing permissions and
+   limitations under the License.
+*)
+module Steel.Actions
+open Steel.Heap
+open Steel.HProp
+open Steel.Memory
+open FStar.Real
+open Steel.Permissions
+module U32 = FStar.UInt32
+
+////////////////////////////////////////////////////////////////////////////////
+// Actions:
+// sel, split, update
+////////////////////////////////////////////////////////////////////////////////
+let pre_action (fp:hprop) (a:Type) (fp':a -> hprop) =
+  hheap fp -> (x:a & hheap (fp' x))
+
+let is_frame_preserving #a #fp #fp' (f:pre_action fp a fp') =
+  forall frame h0.
+    interp (fp `star` frame) h0 ==>
+    (let (| x, h1 |) = f h0 in
+     interp (fp' x `star` frame) h1)
+
+let action_depends_only_on_fp (#pre:_) (#a:_) (#post:_) (f:pre_action pre a post)
+  = forall (h0:hheap pre)
+      (h1:heap {disjoint h0 h1})
+      (post: (x:a -> fp_prop (post x))).
+      (interp pre (join h0 h1) /\ (
+       let (| x0, h |) = f h0 in
+       let (| x1, h' |) = f (join h0 h1) in
+       x0 == x1 /\
+       (post x0 h <==> post x1 h')))
+
+let action (fp:hprop) (a:Type) (fp':a -> hprop) =
+  f:pre_action fp a fp'{ is_frame_preserving f /\
+                         action_depends_only_on_fp f }
+
+
+let pre_m_action (fp:hprop) (a:Type) (fp':a -> hprop) =
+  hmem fp -> (x:a & hmem (fp' x))
+
+val m_action_depends_only_on (#pre:hprop) (#a:Type) (#post:a -> hprop) (f:pre_m_action pre a post) : prop
+
+val is_m_frame_preserving (#a:Type) (#fp:hprop) (#fp':a -> hprop) (f:pre_m_action fp a fp') : prop
+
+let m_action (fp:hprop) (a:Type) (fp':a -> hprop) =
+  f:pre_m_action fp a fp'{ is_m_frame_preserving f /\ m_action_depends_only_on f }
+
+val frame_fp_prop (#fp:_) (#a:Type) (#fp':_) (act:action fp a fp')
+                  (#frame:hprop) (q:fp_prop frame)
+   : Lemma (forall (h0:hheap (fp `star` frame)).
+              (affine_star fp frame h0;
+               q h0 ==>
+               (let (| x, h1 |) = act h0 in
+                q h1)))
